Project2/State.v
@@ -1,0 +1,76 @@
+Require Import Arith ZArith List String.
+Import ListNotations.
+
+(** * Identifiers and Polymorphic States *)
+
+Module Id.
+
+  Inductive t := Id : nat -> t.
+
+  Definition beq (id1 id2:t) : bool :=
+    match (id1, id2) with
+    | (Id n1, Id n2) => beq_nat n1 n2
+    end.
+
+  (** Properties of Id.beq: reflexivity, symmetry. *)
+
+  Fact beq_refl: forall id, beq id id = true.
+  Proof.
+    intros id.
+    destruct id as [ n ].
+    unfold beq.
+    symmetry.
+    apply beq_nat_refl.
+  Qed.
+
+  Fact beq_sym: forall id1 id2, beq id1 id2 = beq id2 id1.
+  Proof.
+    intros id1 id2.
+    destruct id1 as [ n1 ].
+    destruct id2 as [ n2 ].
+    unfold beq.
+    now rewrite Nat.eqb_sym.
+  Qed.
+
+  Fact beq_eq: forall id1 id2,
+      beq id1 id2 = true -> id1 = id2.
+  Proof.
+    intros [ id1 ] [ id2 ] H; unfold beq in *; simpl in *.
+    apply beq_nat_true in H; now rewrite H.
+  Qed.
+  
+End Id.
+
+(** Natural numbers can be understood as identifiers *)
+Coercion Id.Id: nat >-> Id.t.
+
+(** In the module [State], [t A] is the type of a state, i.e.  a
+    partial mapping from identifiers to values of type [A]. *)
+
+Module State.
+
+  Definition t (A:Type)  : Type := list (Id.t * A).
+
+  Definition update{A:Type}(state:t A)(key:Id.t)(value:A):t A :=
+    (key,value)::state.
+
+  Fixpoint find {A:Type}(state:t A)(key:Id.t) : option A :=
+    match state with
+      | [ ] => None
+      | cons (k,v) state' => 
+          if Id.beq key k
+          then Some v
+          else find state' key 
+    end. 
+
+  Fact find_update :
+    forall (A:Type)(k:Id.t) (v:A) (s:t A),
+      find (update s k v) k = Some v.
+  Proof.
+    intros A k v s.
+    simpl.
+    rewrite Id.beq_refl.
+    reflexivity.
+  Qed.
+
+End State.
