Project2/project2.v
@@ -1,27 +1,32 @@
 (* Project 2: *)
 
-Require Import Arith ZArith List String WhileStateFun.
+Require Import Arith ZArith List String State.
 Import ListNotations. 
 
 
 Module Stack.
 
   Inductive A : Type :=
-  | num | inst | empty.
+  | z : Z -> A 
+  | t: bool -> A.
 
-  Inductive t (X:A) : Type := 
-  | nil  : t X
-  | cons : t X -> t X -> t X.
+Inductive t : Type :=
+  | nil : t
+  | cons : A -> t -> t.
 
-  Definition pop stack : A := 
-    match stack with 
-    | a1 :: _ => a1
-    | [ ] => empty
-    end.
-  (* Start of the push function *)
-  (* 
-  Definition push stack (v:A) : Type :=
-   v::stack. *)
+Notation "x :: l" := (cons x l)
+                     (at level 60, right associativity).
+Notation "[ ]" := nil.
+Notation "[ x ; .. ; y ]" := (cons x .. (cons y nil) ..).
+
+Definition push (n:A)(s1:t): t :=
+  cons n s1.
+
+Definition pop (stack:t): t :=
+  match stack with
+  | [ ]  =>  [ ]
+  | _::stack' => stack'
+  end.
 
 End Stack.
 
@@ -42,18 +47,68 @@ Inductive inst: Type :=
 (* Configuration has the form <c,e,s> where c is a sequence of inst, 
     e is the stack, and s is the storage*)
 Inductive configuration : Type :=
-| Rem : inst -> State.t -> configuration
-| Fin : State.t -> configuration.
+| Rem : inst -> State.t Type-> configuration
+| Fin : State.t Type-> configuration.
 
 (** ** Structural Operational Semantics *)
-Inductive am : inst -> State.t -> configuration -> Prop := 
+Inductive am : inst -> State.t Type-> configuration -> Prop := 
 | am_noop:    (* < Skip, s > -> s *)
     forall s, am NOOP s (Fin s)
-| am_fetch: 
-    forall n s, am (State.find n) (Fin s).
-(*| am_push: 
-    forall n, am *)
 
+| am_push: 
+  forall  (n:Z) (s:State.t Type) (e:Stack.t), 
+      am (PUSH n)  s  (Fin (Stack.push n e)).
+
+| am_add: 
+  forall (z1 z2: Z) (s:State.t)  (e:Stack.t), 
+     (Stack.push (ZArith.add Stack.pop Stack.pop))
+
+| am_sub: 
+  forall (z1 z2: Z) (s:State.t)  (e:Stack.t), 
+     (Stack.push (ZArith.sub Stack.pop Stack.pop))
+
+| am_mult: 
+  forall (z1 z2: Z) (s:State.t)  (e:Stack.t), 
+     (Stack.push (ZArith.mult Stack.pop Stack.pop))
+
+| am_fetch: 
+    forall (n:Id.t)  (s:State.t Type) (e:Stack.t), (State.find s n) ::e. 
+
+| am_true: 
+    forall (tt:bool) (s:State.t)  (e:Stack.t), 
+    Stack.push tt e. 
+
+|am_false: 
+   forall (ff:bool) (s:State.t)  (e:Stack.t), 
+    Stack.push ff e.
+
+| am_eq: 
+  forall (z1 z2: Z) (s:State.t)  (e:Stack.t), 
+     (Stack.push (ZArith.eq Stack.pop Stack.pop))
+
+| am_le: 
+  forall (z1 z2: Z) (s:State.t)  (e:Stack.t), 
+     (Stack.push (ZArith.le Stack.pop Stack.pop))
+
+|am_neg_tt: 
+  forall  (c:inst) (s:State.t) (e:Stack.t), 
+  Stack.pop e = tt ->  ff::e 
+
+|am_neg_ff: 
+  forall  (c:inst) (s:State.t) (e:Stack.t), 
+  Stack.pop e = ff -> tt::e 
+
+| am_store: 
+    forall (n:Id.t)  (s:State.t) (e:Stack.t), (State.update (State.find s n) s) .
+
+|am_branch_tt: 
+  forall (c1 c2 c: inst) (e: Stack.t) (s:State.t) , 
+    Stack.pop e = tt ->  c1::c 
+
+|am_branch_ff: 
+  forall (c1 c2 c: inst) (e: Stack.t) (s:State.t) , 
+    Stack.pop e = ff ->  c2::c 
+|am_loop: 
  Module Examples.
 
     Example ex4_1 : t Z :=
